---
title: "Testing"
collection: solutions
type: "Type"
permalink: /jech-solutions/testing
excerpt: ""
---

Main paragraph underscore otherwise, we have $\operatorname{ext}_\in(X) = \operatorname{ext}_\in(\emptyset)$ (note that $\emptyset \in M$ necessary, as we may take any $Y \in M$ and we have $\emptyset = Y - Y \in M$). WLOG suppose $x_{k+1} \in M$.
<ol>
<li>Item underscores $\operatorname{ext}_\in(X) = \operatorname{ext}_\in(\emptyset)$, $Z_a$.</li>
</ol>
    
$$
\operatorname{ext}_\in(X) = \operatorname{ext}_\in(\emptyset)
$$


Main paragraph underscore $\operatorname{ext}\_\in(X) = \operatorname{ext}\_\in(\emptyset)$.
<ol>
<li>Item underscores $\operatorname{ext}\_\in(X) = \operatorname{ext}\_\in(\emptyset)$.
</ol>
    
$$
\operatorname{ext}\_\in(X) = \operatorname{ext}\_\in(\emptyset)
$$