---
title: "2) Ordinal Numbers - Suggested Solutions to Jech's <em>Set Theory</em>"
chapter: "2) Ordinal Numbers"
permalink: /jech-solutions/chapter-2
category: solution
---

{% include commands.html %}

<body>
<a name="ex2.1"></a><br/>
<h2>Exercise 2.1.</h2>
<em>Solution.</em> Suppose $f : P \to Q$ and $g : Q \to R$ are two isomorphisms.<br/>
<br/>
<strong>Reflexive:</strong> The identity $\id : P \to P$ is clearly an isomorphism.<br/>
<br/>
<strong>Symmetry:</strong> By definition of an isomorphism, it's easy to see if $f : P \to Q$ is an isomorphism then so is $f^{-1} : Q \to P$.<br/>
<br/>
<strong>Transitive:</strong> Composition of isomorphisms are isomorphisms, as they remain bijective and:<br/>
$$
\begin{align*}<br/>
x < y \implies f(x) < f(y) \implies g(f(x)) < g(f(y))<br/>
\end{align*}$$
<p align="right">$\square$</p><br/>
<br/>
<a name="ex2.2"></a><br/>
<h2>Exercise 2.2.</h2>
<em>Solution.</em> Note that $\beta < \alpha$ iff $\beta + 1 \leq \alpha$.<br/>
<br/>
<u>$\implies$:</u> Suppose $\beta \in \alpha$. Since $\alpha = \bigcup \alpha$, $\beta \in \gamma$ for some $\gamma \in \alpha$. Then $\beta + 1 \subseteq \gamma$. Since $\gamma \in \alpha$, $\beta + 1 \in \alpha$.<br/>
<br/>
<u>$\impliedby$:</u> If $\beta \in \bigcup \alpha$, then $\beta \in \gamma$ for some $\gamma \in \alpha$. By transitivity of ordinals, $\gamma \subseteq \alpha$, so $\beta \in \alpha$. Thus, $\bigcup \alpha \subseteq \alpha$ (we have not used the hypothesis).<br/>
<br/>
On the other hand, let $\beta \in \alpha$. By hypothesis, $\beta + 1 \in \alpha$, so $\beta + 1 \subseteq \bigcup\alpha$. Hence $\beta \in \bigcup\alpha$.<p align="right">$\square$</p><br/>
<br/>
<a name="ex2.3"></a><br/>
<h2>Exercise 2.3.</h2>
<em>Solution.</em> We shall show that if $A$ and $B$ are inductive, then so is $A \cap B$. Since $\boldsymbol{\mathrm{ORD}}$ is an inductive class, it follows that $X \cap \boldsymbol{\mathrm{ORD}}$ is also inductive.<br/>
<br/>
Clearly $\emptyset \in A \cap B$. Let $x \in A \cap B$. Then since $A$ and $B$ are inductive, $x \cup \lbrace x\rbrace \in A$ and $x \cup \lbrace x\rbrace \in B$, so $x \cup \lbrace x\rbrace \in A \cap B$. Thus $A \cap B$ is inductive.<br/>
<br/>
Since $\boldsymbol{N}$ is the smallest inductive set, $\boldsymbol{N} = \boldsymbol{N} \cap \boldsymbol{\mathrm{ORD}}$, i.e. $\boldsymbol{N} \subseteq \boldsymbol{\mathrm{ORD}}$. Since $\boldsymbol{N}$ is transitive by <a href="https://clementyung.github.io/jech-solutions/chapter-1#ex1.3">Exercise 1.3</a>, and is well-ordered, it is an ordinal.<br/>
<br/>
Finally, to see that $\boldsymbol{N}$ is a limit ordinal, suppose not, so $\boldsymbol{N} = n \cup \lbrace n\rbrace$ for some $n \in \boldsymbol{N}$. By the inductive property of $\boldsymbol{N}$, we have that $\boldsymbol{N} = n \cup \lbrace n\rbrace \in \boldsymbol{N}$, contradicting the Axiom of Regularity.<p align="right">$\square$</p><br/>
<br/>
<a name="ex2.4"></a><br/>
<h2>Exercise 2.4.</h2>
<em>Solution.</em> <u>(i) $\implies$ (ii):</u> If $X$ is inductive, then $\boldsymbol{N} \subseteq X$. Then there exists an injective map $\boldsymbol{N} \to X$, which is the inclusion map. Then $\vert \boldsymbol{N}\vert  \leq \vert X\vert $, so $X$ is infinite.<br/>
<br/>
<u>(ii) $\implies$ (iii):</u> Let $X$ be an infinite set. Consider the map on $[X]^{<\omega}$ (the set of all finite subsets of $X$) defined by:<br/>
$$
\begin{align*}<br/>
Y \mapsto \vert Y\vert <br/>
\end{align*}$$
This is well-defined, as $\vert Y\vert $ is well-defined for finite sets without Axiom of Infinity. By Axiom of Replacement, the image of this map is a set. Since $X$ is infinite, we have that for all $n \in \omega$, there exists $Y \subseteq X$ such that $\vert Y\vert  = n$. Then $Y \mapsto n$, the image of this map is $\omega$. Hence $\omega$ is a set.<br/>
<br/>
<u>(iii) $\implies$ (i):</u> $\omega$ is inductive by definition.<p align="right">$\square$</p><br/>
<br/>
<a name="ex2.5"></a><br/>
<h2>Exercise 2.5.</h2>
<em>Solution.</em> If such a sequence exists, then $\lbrace a_n : n \in \boldsymbol{N}\rbrace \subseteq \boldsymbol{N}$ has no minimal element, contradicting the definition of well-order.<p align="right">$\square$</p><br/>
<br/>
<a name="ex2.6"></a><br/>
<h2>Exercise 2.6.</h2>
<em>Solution.</em> For any ordinal $\alpha$, consider the sequence $\alpha_0 := \alpha$ and $\alpha_{n+1} := \alpha_n + 1$. Let $\beta := \lim_{n \to \omega} \alpha_n$. Then $\beta$ is a limit of a (strictly) increasing sequence of ordinals, and is hence a limit ordinal (as $\bigcup\beta = \beta$).<p align="right">$\square$</p><br/>
<br/>
<a name="ex2.7"></a><br/>
<h2>Exercise 2.7.</h2>
<em>Solution.</em> For any $\alpha_0 \in \boldsymbol{\mathrm{ORD}}$, define $\alpha_{n+1} = \gamma_{\alpha_n}$ as in the hint. Let $\alpha = \lim_{n \to \omega} \alpha_n$. Then, by normality of the sequence:<br/>
$$
\begin{align*}<br/>
\gamma_\alpha = \lim_{n \to \omega} \gamma_{\alpha_n} = \lim_{n \to \omega} \alpha_{n+1} = \alpha<br/>
\end{align*}$$
<p align="right">$\square$</p><br/>
<br/>
<a name="ex2.8"></a><br/>
<h2>Exercise 2.8.</h2>
<a name="lem2.8.A"></a><br/>
<strong>Lemma 2.8.A.</strong> If $\beta$ is a limit ordinal, then so are $\alpha + \beta$, $\alpha \cdot \beta$ and $\alpha^\beta$.<br/>
<br/>
<em>Proof.</em> Let $F(\alpha,\beta)$ denote $\alpha + \beta$, $\alpha \cdot \beta$ or $\alpha^\beta$. In all three cases, we have $F(\alpha,\beta) = \lim_{\xi \to \beta} F(\alpha,\xi)$. Since $F(\alpha,\beta)$ is a limit ordinal iff $F(\alpha,\beta) = \lim_{\delta \to F(\alpha,\beta)} \delta$, it suffices to show that for all $\delta < F(\alpha,\beta)$, there exists some $\xi < \beta$ such that $\delta \leq F(\alpha,\xi$). But this is obviously true, for if $\delta > F(\alpha,\xi)$ for all $\xi < \beta$ then $\delta \geq \lim_{\xi \to \beta} F(\alpha,\xi) = F(\alpha,\beta)$ by definition.<p align="right">$\blacksquare$</p><br/>
<br/>
<a name="ex2.8(i)"></a><br/>
<h3>Exercise 2.8(i).</h3>
<em>Solution.</em> We induct on $\gamma$. For $\gamma = 0$, we have:<br/>
$$
\begin{align*}<br/>
\alpha \cdot (\beta + 0) = \alpha \cdot \beta = \alpha \cdot \beta + \alpha \cdot 0<br/>
\end{align*}$$
Suppose $\gamma = \delta + 1$ and $\alpha \cdot (\beta + \delta) = \alpha \cdot \beta + \alpha \cdot \delta$. Then:<br/>
$$
\begin{align*}<br/>
\alpha \dot (\beta + (\delta + 1)) &= \alpha \dot (\beta + (\delta + 1)) \\<br/>
&= \alpha \cdot ((\beta + \delta) + 1) \\<br/>
&= \alpha \cdot (\beta + \delta) + \alpha \\<br/>
&= (\alpha \cdot \beta + \alpha \cdot \delta) + \alpha && \text{by induction hypothesis} \\<br/>
&= \alpha \cdot \beta + (\alpha \cdot \delta + \alpha) \\<br/>
&= \alpha \cdot \beta + \alpha \cdot (\delta + 1)<br/>
\end{align*}$$
If $\gamma$ is a limit ordinal, then note that $\beta + \gamma$ is also a limit ordinal by <a href="#lem2.8.A">Lemma 2.8.A</a>. Thus:<br/>
$$
\begin{align*}<br/>
\alpha \cdot (\beta + \gamma) &= \alpha \cdot \lim_{\xi \to \gamma} (\beta + \xi) \\<br/>
&= \lim_{\xi \to \gamma} \alpha \cdot (\beta + \xi) \text{} && \text{as $\beta + \gamma$ is limit} \\<br/>
&= \lim_{\xi \to \gamma} (\alpha \cdot \beta + \alpha \cdot \xi) && \text{by induction hypothesis} \\<br/>
&= \alpha \cdot \beta + \lim_{\xi \to \gamma} \alpha \cdot \xi &&\text{as $\alpha \cdot \gamma$ is limit, by Lemma 2.8.A} \\<br/>
&= \alpha \cdot \beta + \alpha \cdot \gamma<br/>
\end{align*}$$
<p align="right">$\square$</p><br/>
<br/>
<a name="ex2.8(ii)"></a><br/>
<h3>Exercise 2.8(ii).</h3>
<em>Solution.</em> We induct on $\gamma$. For $\gamma = 0$, we have:<br/>
$$
\begin{align*}<br/>
\alpha^\beta \cdot \alpha^0 = \alpha^\beta \cdot 1 = \alpha^\beta = \alpha^{\beta + 0}<br/>
\end{align*}$$
Suppose $\gamma = \delta + 1$ and $\alpha^{\beta+\gamma} = \alpha^\beta \cdot \alpha^\gamma$. Then:<br/>
$$
\begin{align*}<br/>
\alpha^{\beta + (\delta + 1)} &= \alpha^{(\beta + \delta) + 1} \\<br/>
&= \alpha^{\beta + \delta} \cdot \alpha \\<br/>
&= (\alpha^\beta \cdot \alpha^\delta) \cdot \alpha && \text{by induction hypothesis} \\<br/>
&= \alpha^\beta \cdot (\alpha^\delta \cdot \alpha) \\<br/>
&= \alpha^\beta \cdot \alpha^{\delta+1}<br/>
\end{align*}$$
Suppose $\gamma$ is a limit ordinal. Then $\alpha^\gamma$ and $\alpha^{\beta+\gamma}$ is a limit ordinal, so:<br/>
$$
\begin{align*}<br/>
\alpha^{\beta+\gamma} &= \lim_{\xi \to \gamma} \alpha^{\beta+\xi} \\<br/>
&= \lim_{\xi \to \gamma} \alpha^\beta \cdot \alpha^\xi && \text{by induction hypothesis} \\<br/>
&= \alpha^\beta \cdot \lim_{\xi \to \gamma} \alpha^\xi && \text{as $\alpha^\gamma$ is a limit ordinal} \\<br/>
&= \alpha^\beta \cdot \alpha^\gamma<br/>
\end{align*}$$
<p align="right">$\square$</p><br/>
<br/>
<a name="ex2.8(iii)"></a><br/>
<h3>Exercise 2.8(iii).</h3>
<em>Solution.</em> We induct on $\gamma$. If $\gamma = 0$, then:<br/>
$$
\begin{align*}<br/>
\alpha^{\beta \cdot 0} = \alpha^0 = 1 = (\alpha^\beta)^0<br/>
\end{align*}$$
If $\gamma = \delta + 1$, then:<br/>
$$
\begin{align*}<br/>
(\alpha^\beta)^{\delta + 1} &= (\alpha^\beta)^\delta \cdot \alpha^\beta \\<br/>
&= \alpha^{\beta \cdot \delta} \cdot \alpha^\beta && \text{by induction hypothesis} \\<br/>
&= \alpha^{\beta \cdot \delta + \beta} && \text{by Exercise 2.8(ii)} \\<br/>
&= \alpha^{\beta \cdot (\delta + 1)}<br/>
\end{align*}$$
If $\gamma$ is a limit ordinal, then:<br/>
$$
\begin{align*}<br/>
(\alpha^\beta)^\gamma &= \lim_{\xi \to \gamma} (\alpha^\beta)^\xi \\<br/>
&= \lim_{\xi \to \gamma} \alpha^{\beta\cdot\xi} && \text{by induction hypothesis} \\<br/>
&= \alpha^{\beta \cdot \gamma} &&\text{as $\beta \cdot \gamma$ is limit, and therefore so is $\alpha^{\beta \cdot \gamma}$}<br/>
\end{align*}$$
<p align="right">$\square$</p><br/>
<br/>
<a name="ex2.9"></a><br/>
<h2>Exercise 2.9.</h2>
<a name="ex2.9(i)"></a><br/>
<h3>Exercise 2.9(i).</h3>
<em>Solution.</em> We first note that:<br/>
$$
\begin{align*}<br/>
1 + \omega = \sup_{n < \omega} (1 + n) = \omega<br/>
\end{align*}$$
Now we have $(\omega + 1) \cdot 2 = \omega + 1 + \omega + 1 = \omega + \omega + 1 = \omega \cdot 2 + 1$. By Lemma 2.25(i), we have $\omega \cdot 2 + 1 < \omega \cdot 2 + 2$.<p align="right">$\square$</p><br/>
<br/>
<a name="ex2.9(ii)"></a><br/>
<h3>Exercise 2.9(ii).</h3>
<em>Solution.</em> Observe that:<br/>
$$
\begin{align*}<br/>
2 \cdot \omega = \sup_{n < \omega} 2 \cdot n = \omega<br/>
\end{align*}$$
We have $(\omega \cdot 2)^2 = \omega \cdot 2 \cdot \omega \cdot 2 = \omega \cdot \omega \cdot 2 = \omega^2 \cdot 2$. By Lemma 2.25(iii), we have that $\omega^2 \cdot 2 < \omega^2 \cdot 4$.<p align="right">$\square$</p><br/>
<br/>
<a name="ex2.10"></a><br/>
<h2>Exercise 2.10.</h2>
<em>Solution.</em> We induct on $\gamma$.<br/>
<br/>
<u>$\alpha + \gamma \leq \beta + \gamma$:</u> If $\gamma = 0$ then this follows from $\alpha < \beta$. If $\gamma = \delta + 1$, then by Lemma 2.25(i) we have that:<br/>
$$
\begin{align*}<br/>
\alpha + \delta \leq \beta + \delta \implies \alpha + \delta + 1 \leq \beta + \delta + 1 \implies \alpha + \gamma \leq \beta + \gamma<br/>
\end{align*}$$
If $\gamma$ is a limit ordinal, then:<br/>
$$
\begin{align*}<br/>
\alpha + \gamma &= \lim_{\xi \to \gamma} (\alpha + \xi) \\<br/>
&\leq \lim_{\xi \to \gamma} (\beta + \xi) && \text{by induction hypothesis} \\<br/>
&= \beta + \gamma<br/>
\end{align*}$$
<u>$\alpha \cdot \gamma \leq \beta \cdot \gamma$:</u> If $\gamma = 0$ then $\alpha \cdot 0 = 0 = \beta \cdot 0$. If $\gamma = \delta + 1$, then:<br/>
$$
\begin{align*}<br/>
\alpha \cdot (\delta + 1) &= \alpha \cdot \delta + \alpha \\<br/>
&\leq \beta \cdot \delta + \alpha && \text{by above and induction hypothesis} \\<br/>
&\leq \beta \cdot \delta + \beta && \text{by $\alpha < \beta$ and Lemma 2.25(i)} \\<br/>
&= \beta \cdot (\delta + 1)<br/>
\end{align*}$$
If $\gamma$ is a limit ordinal, then:<br/>
$$
\begin{align*}<br/>
\alpha \cdot \gamma &= \lim_{\xi \to \gamma} \alpha \cdot \xi \\<br/>
&\leq \lim_{\xi \to \gamma} \beta \cdot \xi && \text{by induction hypothesis} \\<br/>
&= \beta \cdot \gamma<br/>
\end{align*}$$
<u>$\alpha^\gamma \leq \beta^\gamma$:</u> If $\gamma = 0$ then $\alpha^0 = 1 = \beta^0$. If $\gamma = \delta + 1$ then by above and Lemma 2.25:<br/>
$$
\begin{align*}<br/>
\alpha^{\delta+1} &= \alpha^\delta \cdot \alpha \\<br/>
&\leq \beta^\delta \cdot \alpha && \text{by above and induction hypothesis} \\<br/>
&\leq \beta^\delta \cdot \beta && \text{by $\alpha < \beta$ and Lemma 2.25(iii)} \\<br/>
&= \beta^{\delta+1}<br/>
\end{align*}$$
If $\gamma$ is a limit ordinal, then:<br/>
$$
\begin{align*}<br/>
\alpha^\gamma &= \lim_{\xi \to \gamma} \alpha^\xi \\<br/>
&\leq \lim_{\xi \to \gamma} \beta^\xi && \text{by induction hypothesis} \\<br/>
&= \beta^\gamma<br/>
\end{align*}$$
<p align="right">$\square$</p><br/>
<br/>
<a name="ex2.11"></a><br/>
<h2>Exercise 2.11.</h2>
<a name="ex2.11(i)"></a><br/>
<h3>Exercise 2.11(i).</h3>
<em>Solution.</em> As we saw in the proof of <a href="#ex2.9(i)">Exercise 2.9(i)</a>, $0 < 1$ but $0 + \omega = \omega = 1 + \omega$.<p align="right">$\square$</p><br/>
<br/>
<a name="ex2.11(ii)"></a><br/>
<h3>Exercise 2.11(ii).</h3>
<em>Solution.</em> As we saw in the proof of <a href="#ex2.9(ii)">Exercise 2.9(ii)</a>, $1 < 2$ but $1 \cdot \omega = \omega = 2 \cdot \omega$.<p align="right">$\square$</p><br/>
<br/>
<a name="ex2.11(iii)"></a><br/>
<h3>Exercise 2.11(iii).</h3>
<em>Solution.</em> $2 < 3$ but:<br/>
$$
\begin{align*}<br/>
2^\omega = \sup_{n < \omega} 2^n = \omega = \sup_{n < \omega} 3^n = 3^\omega<br/>
\end{align*}$$
<p align="right">$\square$</p><br/>
<br/>
<a name="ex2.12"></a><br/>
<h2>Exercise 2.12.</h2>
<em>Solution.</em> We first show that $\omega^{\varepsilon_0} = \varepsilon_0$. Indeed:<br/>
$$
\begin{align*}<br/>
\omega^{\varepsilon_0} = \lim_{n \to \omega} \omega^{\alpha_n} = \lim_{n \to \omega} \alpha_{n+1} = \varepsilon_0<br/>
\end{align*}$$
Now suppose $\varepsilon$ is another ordinal such that $\omega^\varepsilon = \varepsilon$. Note that $\varepsilon \neq 0$, as $\omega^0 = 1 \neq 0$. Thus, $\varepsilon \geq \omega \alpha_0$. If $\varepsilon \geq \alpha_n$, then by <a href="#ex2.10">Exercise 2.10</a>:<br/>
$$
\begin{align*}<br/>
\alpha_{n+1} = \omega^{\alpha_n} \leq \omega^{\varepsilon} = \varepsilon<br/>
\end{align*}$$
So $\varepsilon \geq \alpha_n$ for all $n$. Thus $\varepsilon$ is an upper bound of the sequence $\c{\alpha_n : n \in \omega}$, so $\varepsilon_0 \leq \varepsilon$.<p align="right">$\square$</p><br/>
<br/>
<a name="ex2.13"></a><br/>
<h2>Exercise 2.13.</h2>
<em>Solution.</em> Call those definitions (i), (ii) and (iii) respectively.<br/>
<br/>
<u>(i) $\implies$ (ii):</u> Let $\alpha < \gamma$. By Lemma 2.25(ii), there exists some $\delta$ such that $\alpha + \delta = \gamma$. Since $\alpha$ is indecomposable, $\delta \geq \gamma$. If $\delta > \gamma$, then by Lemma 2.25(i) and <a href="#ex2.10">Exercise 2.10</a> we have $\alpha + \delta > \alpha + \gamma \geq \gamma$. Thus $\delta = \gamma$.<br/>
<br/>
<u>(ii) $\implies$ (i):</u> For $\alpha < \gamma$ and $\beta < \gamma$, by Lemma 2.25(i) we have $\alpha + \beta < \alpha + \gamma = \gamma$.<br/>
<br/>
<u>(ii) $\implies$ (iii):</u> By Cantor's Normal Form (Theorem 2.26), we may write:<br/>
$$
\begin{align*}<br/>
\gamma = \omega^{\beta_1} \cdot k_1 + \dots + \omega^{\beta_n} \cdot k_n<br/>
\end{align*}$$
where $\gamma \geq \beta_1 > \cdots > \beta_n$, and $k_1,\dots,k_n$ are non-zero natural numbers. Observe that:<br/>
$$
\begin{align*}<br/>
\gamma + \gamma &= \omega^{\beta_1} \cdot k_1 + \dots + \omega^{\beta_n} \cdot k_n + \gamma \\<br/>
&= \omega_{\beta_1} + (\omega^{\beta_1} \cdot (k_1 - 1) + \dots + \omega^{\beta_n} \cdot k_n + \gamma) \\<br/>
&= \omega^{\beta_1} + \gamma<br/>
\end{align*}$$
as $\omega^{\beta_1} \cdot (k_1 - 1) + \dots + \omega^{\beta_n} \cdot k_n < \gamma$ by uniqueness of Cantor's Normal Form. Thus $\gamma = \omega^{\beta_1}$ (i.e. $n = 1$ and $k_1 = 1$).<br/>
<br/>
<u>(iii) $\implies$ (ii):</u> We induct on $\beta$ where $\gamma = \omega^\beta$. If $\beta = 0$, then $\omega^0 = 1$, so the only $\alpha < \gamma$ is $\alpha = 0$, in which then of course $0 + \omega^\beta = \omega^\beta$.<br/>
<br/>
If $\beta = \delta + 1$, then for $\alpha < \gamma$ we write its Cantor's Normal Form $\alpha = \omega^{\beta_1} \cdot k_1 + \dots + \omega^{\beta_n} \cdot k_n$. Since $\alpha < \gamma$, $\beta_1 < \delta + 1$ so $\beta_1 \leq \delta$. Then:<br/>
$$
\begin{align*}<br/>
\alpha + \omega^{\delta+1} &= \omega^{\beta_1} \cdot k_1 + \dots + \omega^{\beta_n} \cdot k_n + \omega^\delta \cdot \omega \\<br/>
&\leq \omega^\delta \cdot (k_1 + \dots + k_n) + \omega^\delta \cdot \omega \\<br/>
&= \omega^\delta \cdot (k_1 + \dots + k_n + \omega) \\<br/>
&= \omega^\delta \cdot \omega \\<br/>
&= \omega^{\delta+1}<br/>
\end{align*}$$
If $\beta$ is a limit ordinal, then for $\alpha < \omega^\beta$ we have that $\alpha < \omega^\xi$ for some $\xi < \beta$. By induction hypothesis, $\alpha + \omega^\xi = \omega^\xi$. Thus we have that $\omega^\beta = \lim_{\xi \to \beta} (\alpha + \omega^\xi) = \lim_{\xi \to \beta} \omega^\xi = \omega^\beta$ for $\alpha < \omega^\beta$.<p align="right">$\square$</p><br/>
<br/>
<a name="ex2.14"></a><br/>
<h2>Exercise 2.14.</h2>
<em>Solution.</em> Suppose such a sequence exists. Consider $X := \lbrace a_n : n \in \boldsymbol{N}\rbrace \subseteq P$. Since $E$ is well-founded, $X$ has some $E$-minimal element, which is $a_n$ for some $n \in \boldsymbol{N}$. Yet $a_n \; E \; a_{n+1}$, a contradiction.<p align="right">$\square$</p><br/>
<br/>
<a name="ex2.15"></a><br/>
<h2>Exercise 2.15.</h2>
<em>Solution.</em> The proof of Theorem 2.15 can be mimicked. Define the function $F$ such that $F(x) = X$ iff there is a sequence $\c{a_y : y \; E \; x}$ (where $a_x := G(\c{a_y : y \; E \; x})$) such that:
<ol>
<li> $(\forall y \; E \; x) \, a_y = F(\c{a_z : z \; E \; y})$.</li>
<li> $x = G(\c{a_y : y \; E \; x})$.</li>
</ol>
The proof of Theorem 2.15 can be followed similarly to show that the $F$ above works.<p align="right">$\square$</p>
</body>